\documentclass{exam}
\usepackage[utf8]{inputenc}

\usepackage{mynotes}

\title{Honours Algebra - Week 1 - Vector Spaces}
\author{Antonio Le√≥n Villares}
\date{January 2022}

\begin{document}

\maketitle

\tableofcontents

\pagebreak

\begin{align*}
   &\begin{pmatrix}\frac{x_1}{x_1} & \frac{x_1}{x_2} & \ldots & \frac{x_1}{x_n} \end{pmatrix} 
   \begin{pmatrix}
   a_{1k} \\
   a_{2k} \\
   \vdots \\
   a_{kk} \\
   \vdots \\
   a_{kn}
   \end{pmatrix}
   \\
   =& x_1 \sum_{i = 1}^n \frac{1}{x_i}a_{ik}
\end{align*}

From definition, if $i \neq k$:
\[
\frac{1}{x_i}a_{ik} = \frac{1}{x_i}\frac{x_i}{x_i - x_k} = \frac{1}{x_i - x_k}
\]
and if $i = k$:
\[
\frac{1}{x_i}a_{ik} = \frac{1}{x_k}a_{kk} = \frac{1}{x_k}\sum_{j = 1, j \neq k}^n\frac{x_k}{x_k - x_j} = \sum_{j = 1, j \neq k}^n\frac{1}{x_k - x_j}
\]
So we have:
\begin{align*}
    \vec{v}_1\vec{A}_k &= x_1 \sum_{i = 1}^n \frac{1}{x_i}a_{ik} \\
                       &= x_1 \left(\sum_{i = 1, i \neq k}^n \frac{1}{x_i - x_k} + \sum_{j = 1, j \neq k}^n\frac{1}{x_k - x_j}\right) \\
                       &= x_1 \left(\sum_{i = 1, i \neq k}^n \frac{1}{x_i - x_k} - \sum_{j = 1, j \neq k}^n\frac{1}{x_j - x_k}\right) \\
                       &= x_1 \left(\sum_{i = 1, i \neq k}^n \frac{1}{x_i - x_k} - \sum_{i = 1, i \neq k}^n\frac{1}{x_i - x_k}\right) \\
                       &= 0
\end{align*}

\begin{align*}
    \vec{v}_n\vec{A}_k &= \begin{pmatrix}1 & 1 & \ldots & 1 \end{pmatrix} 
    \begin{pmatrix}
   a_{1k} \\
   a_{2k} \\
   \vdots \\
   a_{kk} \\
   \vdots \\
   a_{kn}
   \end{pmatrix}
   \\
   &= \sum_{i = 1}^n a_{ik} \\
   &= \sum_{i = 1, i \neq k}^n \frac{x_i}{x_i - x_k} + \sum_{j = 1, j \neq k}^n\frac{x_k}{x_k - x_j} \\
   &= \sum_{i = 1, i \neq k}^n \frac{x_i}{x_i - x_k} - \sum_{i = 1, i \neq k}^n\frac{x_k}{x_i - x_k} \\
   &= \sum_{i = 1, i \neq k}^n \frac{x_i - x_k}{x_i - x_k}  \\
   &= n-1  \\
\end{align*}
where we use the fact that $i \neq k$, and each $x$ is pairwise distinct, so $x_i - x_k \neq 0$; alongside the fact that we are adding $\frac{x_i - x_k}{x_i - x_k} = 1$ $n - 1$ times (since we ignore when $i = k$)

\begin{align*}
    \sum_{j = 1, j \neq k}^n \frac{v_jx_j - v_kx_k}{x_j - x_k} &= \sum_{j = 1, j \neq k}^n \frac{x_j\left(\frac{\sum_{b = 1, b \neq j}^n x_b}{\sum_{b = 2}^n x_b}\right) - x_k\left(\frac{\sum_{b = 1, b \neq k}^n x_b}{\sum_{b = 2}^n x_b}\right)}{x_j - x_k} \\
    &= \sum_{j = 1, j \neq k}^n \frac{(x_j - x_k)\left(\frac{\sum_{b = 1, b \neq j, b \neq k}^n x_b}{\sum_{b = 2}^n x_b}\right)}{x_j - x_k} \\
    &= \sum_{j = 1, j \neq k}^n \frac{\sum_{b = 1, b \neq j, b \neq k}^n x_b}{\sum_{b = 2}^n x_b} \\
    &= \frac{1}{\sum_{b = 2}^n x_b}\sum_{j = 1, j \neq k}^n \sum_{b = 1, b \neq j, b \neq k}^n x_b \\
\end{align*}

\end{document}